getting ready to use the monadic version of chain

src/tidy/profiling.lean
@@ -1,38 +1,14 @@
+-- Copyright (c) 2017 Scott Morrison. All rights reserved.
+-- Released under Apache 2.0 license as described in the file LICENSE.
+-- Authors: Scott Morrison
+
+import .tactic_states
 import .if_then_else
 import .tidy
 
 open tactic
 
-universe variables u v w
-
-meta class underlying_tactic_state ( σ : Type ) :=
-  ( to_tactic_state : σ → tactic_state )
-
-meta instance underlying_tactic_state_coe (σ : Type) [underlying_tactic_state σ] : has_coe σ tactic_state :=
-⟨ underlying_tactic_state.to_tactic_state ⟩
-
-meta instance trivial_underlying_tactic_state : underlying_tactic_state tactic_state :=
-{ to_tactic_state := id }
-
-meta instance product_underlying_tactic_state ( σ τ : Type ) [underlying_tactic_state σ]: underlying_tactic_state (σ × τ) :=
-{ to_tactic_state := λ p, underlying_tactic_state.to_tactic_state p.1 }
-
-meta class tactic_lift ( τ : Type ) :=
-  ( lift : Π { σ α : Type } [underlying_tactic_state σ], interaction_monad σ α → interaction_monad (σ × τ) α )
-
-meta instance tactic_lift_coe (τ : Type) [tactic_lift τ] (σ α : Type) [underlying_tactic_state σ] : has_coe (interaction_monad σ α) (interaction_monad (σ × τ) α) :=
-⟨ tactic_lift.lift τ ⟩
-
-meta instance interaction_monad.has_orelse (σ : Type) : has_orelse (interaction_monad σ) := {
-  orelse := λ { α : Type } (t₁ t₂ : interaction_monad σ α) s, 
-              match (t₁ s) with
-              | result.success   a       s' := result.success a s'
-              | result.exception msg pos s' := match (t₂ s') with
-                                               | result.success   a'        s'' := result.success   a'        s''
-                                               | result.exception msg' pos' s'' := result.exception msg' pos' s''
-                                               end
-              end
-}
+universe variables u v
 
 --- Profiling:
 
@@ -87,67 +63,3 @@ success_if_fail { profiling $ done <|> done }, -- 2
 
 triv
 end
-
-structure loop_detection_state := 
-  ( past_goals : list string )
-
-meta def unreachable {α : Sort u} : α := undefined_core "unreachable"
-
-meta def detect_looping
-  { σ α : Type } 
-  [ underlying_tactic_state σ ]
-  ( t : interaction_monad (σ × loop_detection_state) α ) 
-    : interaction_monad σ α :=
-λ s, match (hash_target s) with
-     | result.success   hash    s' := match t (s, ⟨ [ hash ] ⟩ ) with
-                                      | result.success a s''         := result.success a s''.1
-                                      | result.exception pos msg s'' := result.exception pos msg (s''.1)
-                                      end
-     | result.exception pos msg s' := unreachable
-     end
-
-meta instance lift_to_loop_detection_tactic : tactic_lift loop_detection_state := 
-{
-  lift := λ { σ α : Type } [uts : underlying_tactic_state σ] ( t : interaction_monad σ α ) (s : σ × loop_detection_state),
-            match t s.1 with
-            | result.success   a       s' := match (hash_target (@underlying_tactic_state.to_tactic_state _ uts s')) with -- FIXME why doesn't the coercion work? why can't Lean find uts itself?
-                                             | result.success hash s'' := if s.2.past_goals.mem hash then
-                                                                            match (@tactic.fail α string _ ("detected looping\n" ++ s.2.past_goals.to_string ++ "\n" ++ hash)) s'' with -- FIXME this duplicates code above
-                                                                            | result.success   a       s''' := unreachable
-                                                                            | result.exception pos msg s''' := result.exception pos msg (s', s.2)
-                                                                            end
-                                                                          else  
-                                                                            result.success a (s', ⟨ hash :: s.2.past_goals ⟩ )
-                                             | _ := unreachable
-                                             end
-            | result.exception msg pos s' := result.exception msg pos (s', s.2)
-            end
-} 
-
-meta def simp := `[simp]
-
-lemma looping_test_1 (a : empty): 1 = 1 :=
-begin
-success_if_fail { detect_looping $ skip },
-success_if_fail { detect_looping $ skip >> skip },
-refl
-end
-lemma looping_test_2 (a : empty): 1 = 1 :=
-begin
-detect_looping $ simp
-end
-
--- Lean won't chain two coercions together for us, so we provide a shortcut here.
-meta instance tactic_lift_twice_coe (τ τ' : Type) [tactic_lift τ] [tactic_lift τ'] (σ α : Type) [underlying_tactic_state σ] : has_coe (interaction_monad σ α) (interaction_monad ((σ × τ) × τ') α) :=
-⟨ λ t, tactic_lift.lift τ' (tactic_lift.lift τ t) ⟩
-
-lemma looping_and_profiling_at_the_same_time_test_1 : true :=
-begin
-profiling $ (detect_looping $ triv),
-end
-lemma looping_and_profiling_at_the_same_time_test_2 : true :=
-begin
-success_if_fail { profiling $ detect_looping $ skip >> skip },
-triv
-end
-
