src/tidy/loop_detection.lean
@@ -1,0 +1,74 @@
+-- Copyright (c) 2017 Scott Morrison. All rights reserved.
+-- Released under Apache 2.0 license as described in the file LICENSE.
+-- Authors: Scott Morrison
+
+import .profiling
+
+open tactic
+
+universe variables u v
+
+
+structure loop_detection_state := 
+  ( past_goals : list string )
+
+meta def unreachable {α : Sort u} : α := undefined_core "unreachable"
+
+meta def detect_looping
+  { σ α : Type } 
+  [ underlying_tactic_state σ ]
+  ( t : interaction_monad (σ × loop_detection_state) α ) 
+    : interaction_monad σ α :=
+λ s, match (hash_target s) with
+     | result.success   hash    s' := match t (s, ⟨ [ hash ] ⟩ ) with
+                                      | result.success a s''         := result.success a s''.1
+                                      | result.exception pos msg s'' := result.exception pos msg (s''.1)
+                                      end
+     | result.exception pos msg s' := unreachable
+     end
+
+meta instance lift_to_loop_detection_tactic : tactic_lift loop_detection_state := 
+{
+  lift := λ { σ α : Type } [uts : underlying_tactic_state σ] ( t : interaction_monad σ α ) (s : σ × loop_detection_state),
+            match t s.1 with
+            | result.success   a       s' := match (hash_target (@underlying_tactic_state.to_tactic_state _ uts s')) with -- FIXME why doesn't the coercion work? why can't Lean find uts itself?
+                                             | result.success hash s'' := if s.2.past_goals.mem hash then
+                                                                            match (@tactic.fail α string _ ("detected looping\n" ++ s.2.past_goals.to_string ++ "\n" ++ hash)) s'' with -- FIXME this duplicates code above
+                                                                            | result.success   a       s''' := unreachable
+                                                                            | result.exception pos msg s''' := result.exception pos msg (s', s.2)
+                                                                            end
+                                                                          else  
+                                                                            result.success a (s', ⟨ hash :: s.2.past_goals ⟩ )
+                                             | _ := unreachable
+                                             end
+            | result.exception msg pos s' := result.exception msg pos (s', s.2)
+            end
+} 
+
+meta def simp := `[simp]
+
+lemma looping_test_1 (a : empty): 1 = 1 :=
+begin
+success_if_fail { detect_looping $ skip },
+success_if_fail { detect_looping $ skip >> skip },
+refl
+end
+lemma looping_test_2 (a : empty): 1 = 1 :=
+begin
+detect_looping $ simp
+end
+
+-- Lean won't chain two coercions together for us, so we provide a shortcut here.
+meta instance tactic_lift_twice_coe (τ τ' : Type) [tactic_lift τ] [tactic_lift τ'] (σ α : Type) [underlying_tactic_state σ] : has_coe (interaction_monad σ α) (interaction_monad ((σ × τ) × τ') α) :=
+⟨ λ t, tactic_lift.lift τ' (tactic_lift.lift τ t) ⟩
+
+lemma looping_and_profiling_at_the_same_time_test_1 : true :=
+begin
+profiling $ (detect_looping $ triv),
+end
+lemma looping_and_profiling_at_the_same_time_test_2 : true :=
+begin
+success_if_fail { profiling $ detect_looping $ skip >> skip },
+triv
+end
+
