src/tidy/monadic_chain.lean
@@ -1,14 +1,15 @@
 import .if_then_else
+import .tactic_states
 
-private meta structure chain_progress ( α : Type ) ( m : Type → Type ) [monad m] :=
+private meta structure chain_progress ( σ α : Type ) :=
   ( iteration_limit   : nat )
   ( results           : list α )
-  ( remaining_tactics : list (m α) )
+  ( remaining_tactics : list (interaction_monad (tactic_state × σ) α) )
 
 open nat tactic
 
-private meta def chain' { α : Type } { m : Type → Type } [monad m] [has_orelse m] ( tactics : list (m α) ) 
-    : chain_progress α m → m (list α)
+private meta def chain' { σ α : Type } [ tactic_lift σ ] ( tactics : list (interaction_monad (tactic_state × σ) α) ) 
+    : chain_progress σ α → interaction_monad (tactic_state × σ) (list α)
 | ⟨ 0     , _      , _       ⟩ := fail "chain iteration limit exceeded"
 | ⟨ _     , results, []      ⟩ := pure results
 | ⟨ succ n, results, t :: ts ⟩ := if_then_else done
