src/tidy/tactic_states.lean
@@ -1,0 +1,36 @@
+-- Copyright (c) 2017 Scott Morrison. All rights reserved.
+-- Released under Apache 2.0 license as described in the file LICENSE.
+-- Authors: Scott Morrison
+
+open tactic
+
+universe variables u v w
+
+meta class underlying_tactic_state ( σ : Type ) :=
+  ( to_tactic_state : σ → tactic_state )
+
+meta instance underlying_tactic_state_coe (σ : Type) [underlying_tactic_state σ] : has_coe σ tactic_state :=
+⟨ underlying_tactic_state.to_tactic_state ⟩
+
+meta instance trivial_underlying_tactic_state : underlying_tactic_state tactic_state :=
+{ to_tactic_state := id }
+
+meta instance product_underlying_tactic_state ( σ τ : Type ) [underlying_tactic_state σ]: underlying_tactic_state (σ × τ) :=
+{ to_tactic_state := λ p, underlying_tactic_state.to_tactic_state p.1 }
+
+meta class tactic_lift ( τ : Type ) :=
+  ( lift : Π { σ α : Type } [underlying_tactic_state σ], interaction_monad σ α → interaction_monad (σ × τ) α )
+
+meta instance tactic_lift_coe (τ : Type) [tactic_lift τ] (σ α : Type) [underlying_tactic_state σ] : has_coe (interaction_monad σ α) (interaction_monad (σ × τ) α) :=
+⟨ tactic_lift.lift τ ⟩
+
+meta instance interaction_monad.has_orelse (σ : Type) : has_orelse (interaction_monad σ) := {
+  orelse := λ { α : Type } (t₁ t₂ : interaction_monad σ α) s, 
+              match (t₁ s) with
+              | result.success   a       s' := result.success a s'
+              | result.exception msg pos s' := match (t₂ s') with
+                                               | result.success   a'        s'' := result.success   a'        s''
+                                               | result.exception msg' pos' s'' := result.exception msg' pos' s''
+                                               end
+              end
+}
